module Calculus.PolyLinear.Rules.Weakening where

open import Calculus.PolyLinear.Syntax
open import Calculus.PolyLinear.Syntax.Properties
open import Calculus.PolyLinear.Rules
open import Data.List
open import Data.Nat
open import Data.Nat.Properties
open import Data.Product
open import Relation.Binary.PropositionalEquality
open import Relation.Nullary
open import Relation.Nullary.Decidable

𝕂∈⇒len+𝕂∈++ : x ⦂ K 𝕂∈ Γ′ → len Δ + x ⦂ wk∣ len Δ ↑ 0 ∣ K 𝕂∈ Δ ++ Γ′
𝕂∈⇒len+𝕂∈++ {K = K} {Δ = []}    x∈
  rewrite wk𝕂∣0↑x∣≡id K 0          = x∈
𝕂∈⇒len+𝕂∈++ {K = K} {Δ = _ ∷ _} x∈ = there (𝕂∈⇒len+𝕂∈++ x∈)

𝕋∈⇒len+𝕋∈++ : x ⦂ T 𝕋∈ Γ′ / Γ″ → len Δ + x ⦂ wk∣ len Δ ↑ 0 ∣ T 𝕋∈ Δ ++ Γ′ / Δ ++ Γ″
𝕋∈⇒len+𝕋∈++ {T = T} {Δ = []}    x∈
  rewrite wk𝕋∣0↑x∣≡id T 0          = x∈
𝕋∈⇒len+𝕋∈++ {T = T} {Δ = _ ∷ _} x∈ = {!!} -- requires weakening decomposition

≥len⇒𝕂∈++⇒len+𝕂∈++-++ : ∀ Γ → x ≥ len Γ → x ⦂ K 𝕂∈ Γ ++ Γ′ → len Δ + x ⦂ wk∣ len Δ ↑ 0 ∣ K 𝕂∈ wk∣ len Δ ↑ len Γ ∣ Γ ++ Δ ++ Γ′
≥len⇒𝕂∈++⇒len+𝕂∈++-++                     []      z≤n      x∈         = 𝕂∈⇒len+𝕂∈++ x∈
≥len⇒𝕂∈++⇒len+𝕂∈++-++ {x = suc x} {Δ = Δ} (_ ∷ Γ) (s≤s x≥) (there x∈)
  rewrite +-suc (len Δ) x                                             = there (≥len⇒𝕂∈++⇒len+𝕂∈++-++ Γ x≥ x∈)

<len⇒𝕂∈++⇒len+𝕂∈++-++ : ∀ Γ → x < len Γ → x ⦂ K 𝕂∈ Γ ++ Γ′ → x ⦂ wk∣ len Δ ↑ len Γ ∣ K 𝕂∈ wk∣ len Δ ↑ len Γ ∣ Γ ++ Δ ++ Γ′
<len⇒𝕂∈++⇒len+𝕂∈++-++ (_ ∷ Γ) x<       (here refl) = here refl
<len⇒𝕂∈++⇒len+𝕂∈++-++ (_ ∷ Γ) (s≤s x<) (there x∈)  = there (<len⇒𝕂∈++⇒len+𝕂∈++-++ Γ x< x∈)

wk∣↑∣𝕂∈ : ∀ Γ →
          x ⦂ K 𝕂∈ Γ ++ Γ′ →
          --------------------------------------------
          wk∣ len Δ ↑ len Γ ∣ x ⦂ wk∣ len Δ ↑ len Γ ∣ K 𝕂∈ wk∣ len Δ ↑ len Γ ∣ Γ ++ Δ ++ Γ′
wk∣↑∣𝕂∈ {x} []               x∈
  rewrite proj₂ (dec-yes (x ≥? 0) z≤n) = 𝕂∈⇒len+𝕂∈++ x∈
wk∣↑∣𝕂∈ {x} (K       /𝕂 ∷ Γ) x∈
  with x ≥? suc (len Γ)
...  | yes x≥                          = ≥len⇒𝕂∈++⇒len+𝕂∈++-++ (_ ∷ Γ) x≥ x∈
...  | no  x≱                          = <len⇒𝕂∈++⇒len+𝕂∈++-++ (_ ∷ Γ) (≰⇒> x≱) x∈
wk∣↑∣𝕂∈ {x} ((T , u) /𝕋 ∷ Γ) x∈
  with x ≥? suc (len Γ)
...  | yes x≥                          = ≥len⇒𝕂∈++⇒len+𝕂∈++-++ (_ ∷ Γ) x≥ x∈
...  | no  x≱                          = <len⇒𝕂∈++⇒len+𝕂∈++-++ (_ ∷ Γ) (≰⇒> x≱) x∈

wk∣↑∣𝕋∈ : ∀ Γ →
          x ⦂ T 𝕋∈ Γ ++ Γ′ / Γ₀ →
          --------------------------------------------
          let Γ″ , Γ‴ = splitAt (len Γ) Γ₀ in
          wk∣ len Δ ↑ len Γ ∣ x ⦂ wk∣ len Δ ↑ len Γ ∣ T 𝕋∈ wk∣ len Δ ↑ len Γ ∣ Γ ++ Δ ++ Γ′ / wk∣ len Δ ↑ len Γ ∣ Γ″ ++ Δ ++ Γ‴
wk∣↑∣𝕋∈ {x} []               x∈
  rewrite proj₂ (dec-yes (x ≥? 0) z≤n) = 𝕋∈⇒len+𝕋∈++ x∈
wk∣↑∣𝕋∈ {x} (K       /𝕂 ∷ Γ) x∈
  with x ≥? suc (len Γ)
...  | yes x≥                          = {!!} -- ≥len⇒𝕂∈++⇒len+𝕂∈++-++ (_ ∷ Γ) x≥ x∈
...  | no  x≱                          = {!!} -- <len⇒𝕂∈++⇒len+𝕂∈++-++ (_ ∷ Γ) (≰⇒> x≱) x∈
wk∣↑∣𝕋∈ {x} ((T , u) /𝕋 ∷ Γ) x∈
  with x ≥? suc (len Γ)
...  | yes x≥                          = {!!} -- ≥len⇒𝕂∈++⇒len+𝕂∈++-++ (_ ∷ Γ) x≥ x∈
...  | no  x≱                          = {!!} -- <len⇒𝕂∈++⇒len+𝕂∈++-++ (_ ∷ Γ) (≰⇒> x≱) x∈

𝕋⊢wk∣↑∣ : ∀ Γ →
          ℂ⊢ Δ ++ Γ′ →
          Γ ++ Γ′ 𝕋⊢ T ⦂ K →
          --------------------------------------------
          wk∣ len Δ ↑ len Γ ∣ Γ ++ Δ ++ Γ′ 𝕋⊢ wk∣ len Δ ↑ len Γ ∣ T ⦂ wk∣ len Δ ↑ len Γ ∣ K
ℂ⊢wk∣↑∣ : ∀ Γ →
          ℂ⊢ Δ ++ Γ′ →
          ℂ⊢ Γ ++ Γ′ →
          ---------------
          ℂ⊢ wk∣ len Δ ↑ len Γ ∣ Γ ++ Δ ++ Γ′

𝕋⊢wk∣↑∣ Γ ⊢ΔΓ′ (tvarₗ ⊢ΓΓ′ x∈) = tvarₗ (ℂ⊢wk∣↑∣ Γ ⊢ΔΓ′ ⊢ΓΓ′) (wk∣↑∣𝕂∈ Γ x∈)
𝕋⊢wk∣↑∣ Γ ⊢ΔΓ′ (⊢T ⊸ₗ ⊢U)      = 𝕋⊢wk∣↑∣ Γ ⊢ΔΓ′ ⊢T ⊸ₗ 𝕋⊢wk∣↑∣ Γ ⊢ΔΓ′ ⊢U
𝕋⊢wk∣↑∣ Γ ⊢ΔΓ′ (!ₗ ⊢T)         = !ₗ (𝕋⊢wk∣↑∣ Γ ⊢ΔΓ′ ⊢T)
𝕋⊢wk∣↑∣ Γ ⊢ΔΓ′ (∀ₗ⋆∙ ⊢T)       = ∀ₗ⋆∙ (𝕋⊢wk∣↑∣ (_ ∷ Γ) ⊢ΔΓ′ ⊢T)

ℂ⊢wk∣↑∣ []               ⊢ΔΓ′ ⊢ΓΓ′           = ⊢ΔΓ′
ℂ⊢wk∣↑∣ (K       /𝕂 ∷ Γ) ⊢ΔΓ′ (⋆/𝕂   ∷ ⊢ΓΓ′) = ⋆/𝕂 ∷ ℂ⊢wk∣↑∣ Γ ⊢ΔΓ′ ⊢ΓΓ′
ℂ⊢wk∣↑∣ ((T , u) /𝕋 ∷ Γ) ⊢ΔΓ′ (⊢T /𝕋 ∷ ⊢ΓΓ′) = 𝕋⊢wk∣↑∣ Γ ⊢ΔΓ′ ⊢T /𝕋 ∷ ℂ⊢wk∣↑∣ Γ ⊢ΔΓ′ ⊢ΓΓ′

𝕄⊢wk∣↑∣ : ∀ Γ →
          ℂ⊢ Δ ++ Γ′ →
          Γ ++ Γ′ 𝕄⊢ M ⦂ T / Γ₀ →
          --------------------------------------------
          let Γ″ , Γ‴ = splitAt (len Γ) Γ₀ in
          wk∣ len Δ ↑ len Γ ∣ Γ ++ Δ ++ Γ′ 𝕄⊢ wk∣ len Δ ↑ len Γ ∣ M ⦂ wk∣ len Δ ↑ len Γ ∣ T / wk∣ len Δ ↑ len Γ ∣ Γ″ ++ Δ ++ Γ‴
𝕄⊢wk∣↑∣ Γ ⊢ΔΓ′ (varₗ x) = varₗ {!!}
𝕄⊢wk∣↑∣ Γ ⊢ΔΓ′ (λₗ ⊢T ∘ ⊢M) = λₗ 𝕋⊢wk∣↑∣ Γ ⊢ΔΓ′ ⊢T ∘ {!𝕄⊢wk∣↑∣ (_ ∷ Γ) ⊢ΔΓ′ ⊢M!} -- requires weakening exchange
𝕄⊢wk∣↑∣ Γ ⊢ΔΓ′ (⊢M $ₗ∘ ⊢N) = 𝕄⊢wk∣↑∣ Γ ⊢ΔΓ′ ⊢M $ₗ∘ {!𝕄⊢wk∣↑∣ Γ ⊢ΔΓ′ ⊢N!}
𝕄⊢wk∣↑∣ Γ ⊢ΔΓ′ (bangₗ ⊢M) = {!!}
𝕄⊢wk∣↑∣ Γ ⊢ΔΓ′ (let-bangₗ ⊢M inₗ ⊢N) = let-bangₗ 𝕄⊢wk∣↑∣ Γ ⊢ΔΓ′ ⊢M inₗ {!!}
𝕄⊢wk∣↑∣ Γ ⊢ΔΓ′ (Λₗ⋆∙ ⊢M) = Λₗ⋆∙ 𝕄⊢wk∣↑∣ (_ ∷ Γ) ⊢ΔΓ′ ⊢M
𝕄⊢wk∣↑∣ Γ ⊢ΔΓ′ (⊢M $$ₗ∙ ⊢T) = {!!} -- requires weakening over substitution
